NLustre/CoindToNatmap.v
@@ -1,0 +1,95 @@
+Require Import List.
+Import List.ListNotations.
+Open Scope list_scope.
+Require Import Coq.Sorting.Permutation.
+Require Import Morphisms.
+
+Require Import Coq.FSets.FMapPositive.
+Require Import Velus.Common.
+Require Import Velus.Operators.
+Require Import Velus.Clocks.
+Require Import Velus.NLustre.NLSyntax.
+Require Import Velus.NLustre.Ordered.
+Require Import Velus.NLustre.Stream.
+Require Import Velus.NLustre.Streams.
+
+Require Import Velus.NLustre.NLSemantics.
+Require Import Velus.NLustre.NLSemanticsCoInd.
+
+Require Import Setoid.
+Module Type COINDTONATMAP
+       (Import Ids   : IDS)
+       (Import Op    : OPERATORS)
+       (Import OpAux : OPERATORS_AUX Op)
+       (Import Clks  : CLOCKS    Ids)
+       (Import Syn   : NLSYNTAX  Ids Op Clks)
+       (Import Str   : STREAM        Op OpAux)
+       (Import Ord   : ORDERED   Ids Op Clks Syn)
+       (Sem          : NLSEMANTICS Ids Op OpAux Clks Syn Str Ord)
+       (Mod          : NLSEMANTICSCOIND Ids Op OpAux Clks Syn Ord).
+
+  Section Global.
+
+    Variable G : global.
+
+    Fixpoint to_map {A} (xss: list (Stream A)) : stream (list A) :=
+      match xss with
+      | [] => fun n => []
+      | xs :: xss => fun n => Str_nth n xs :: to_map xss n
+      end.
+
+    Definition hist_to_map (H: Mod.history) : Sem.history :=
+      PM.map (fun xs => fun n => Str_nth n xs) H.
+
+    Lemma sem_var_impl:
+      forall H b xs xss,
+      Forall2 (Mod.sem_var H) xs xss ->
+      Sem.sem_vars b (hist_to_map H) xs (to_map xss).
+    Proof.
+      induction 1 as [|? ? ? ? Find];
+        simpl; unfold Sem.sem_vars, Sem.lift; auto.
+      intro; constructor; auto.
+      constructor.
+      inv Find.
+      unfold Sem.restr, hist_to_map.
+      unfold PM.map.
+      rewrite 2 PM.gmapi.
+      erewrite PM.find_1; eauto; simpl.
+      f_equal.
+      apply eqst_ntheq; symmetry; auto.
+    Qed.
+
+    Theorem implies:
+      forall f xss oss,
+        Mod.sem_node G f xss oss ->
+        Sem.sem_node G f (to_map xss) (to_map oss).
+    Proof.
+      intros ** Sem.
+      induction Sem as [
+                      |
+                      |
+                      |
+                      |
+                      | ? ? ? ? ? Find]
+                         using Mod.sem_node_mult with
+          (P_equation := fun H b e => True)
+          (P_reset := fun f r xss oss => True).
+      - auto.
+      - auto.
+      - auto.
+      - auto.
+      - auto.
+      - econstructor; eauto.
+        + apply Sem.clock_of_equiv.
+        + apply sem_var_impl; eauto.
+        + apply sem_var_impl; eauto.
+        + admit.
+        + admit.
+        + admit.
+        + admit.
+    Qed.
+
+
+  End Global.
+
+End COINDTONATMAP.
